implement protocol

bce/service.dfy
@@ -38,15 +38,42 @@ predicate serviceExchangeSymbols(s: Service, s': Service)
     && s' == s.(nodes := s'.nodes, state := SPhase2)
     && |s'.nodes| == |s.nodes|
     && forall id :: 0 <= id < |s.nodes| ==> 
-        assert symbolsForExchange[id][id] == s.nodes[id].codeword[id];
+        // assert symbolsForExchange[id][id] == s.nodes[id].codeword[id];  // TODO
         nodeReceiveSymbols(s.nodes[id], s'.nodes[id], symbolsForExchange[id])
 }
 
-
-predicate serviceNext(s:Service, s':Service)
+predicate serviceExchangeSyndromesAndDecide(s: Service, s': Service) 
+    requires s.state == SPhase2
+    requires s.f > 0;
+    requires s.n == 3*s.f + 1;
+    requires |s.nodes| == s.n;
+    requires forall sn :: sn in s.nodes ==> sn.n == s.n;
+    requires forall sn :: sn in s.nodes ==> sn.f == s.f;
+    requires forall sn :: sn in s.nodes ==> 0 <= sn.id < s.n;
+    requires forall sn :: sn in s.nodes ==> s.n == |sn.symbols| == |sn.codeword|;
+    requires forall sn :: sn in s.nodes ==> sn.state == Phase2;
+    // requires forall sn :: sn in s.nodes ==> sn.codeword[sn.id] == sn.symbols[sn.id];
 {
-    // TODO
-    true
+    var syndromesForExchange := syndromesToExchange(s.nodes);
+    lemma_Exchanged_Syndromes_Are_Extracted(s.nodes);
+
+    && s' == s.(nodes := s'.nodes, state := SDecided)
+    && |s'.nodes| == |s.nodes|
+    && forall id :: 0 <= id < |s.nodes| ==> 
+    // assert s.nodes[id].codeword[id] == s.nodes[id].symbols[id];
+        nodeReceiveSyndromesAndDecide(s.nodes[id], s'.nodes[id], syndromesForExchange[id])
+}
+
+
+predicate BCE(s:Service, s':Service, s'':Service)
+{
+    if serviceInit(s) then
+        lemma_Exchanged_Symbols_Are_Extracted(s.nodes);
+        && serviceInit(s)
+        && serviceExchangeSymbols(s, s')
+        && serviceExchangeSyndromesAndDecide(s', s'')
+    else 
+        false
 }
 
 
@@ -90,6 +117,50 @@ function extractSymbols(nodes: seq<Node>) : seq<symbol>
     [nodes[0].codeword[nodes[0].id]] + extractSymbols(nodes[1..])
 }
 
+
+
+/* Helper function for SPhase2 -> SDecided transition. 
+* syndromeToExchange(nodes)[i] represents the seq of syndromes that nodes[i] receives in 
+* the exhange phase */
+function syndromesToExchange(nodes: seq<Node>) : seq<seq<syndrome>> 
+    requires forall s :: s in nodes ==> |nodes| == s.n == 3*s.f + 1;
+    requires forall s :: s in nodes ==> 0 <= s.id < s.n;
+    requires forall s :: s in nodes ==> s.n == |s.symbols| == |s.codeword|;
+    requires forall s :: s in nodes ==> s.state == Phase2;
+    // requires forall s :: s in nodes ==> s.codeword[s.id] == s.symbols[s.id];
+{
+    syndromesToExchangeHelper(nodes, 0)
+}
+
+
+function syndromesToExchangeHelper(nodes: seq<Node>, i: nat) : seq<seq<syndrome>> 
+    decreases |nodes| - i;
+    requires 0 <= i <= |nodes|;
+    requires forall s :: s in nodes ==> s.n == 3*s.f + 1;
+    requires forall s :: s in nodes ==> 0 <= s.id < s.n;
+    requires forall s :: s in nodes ==> s.n == |s.symbols| == |s.codeword|;
+    requires forall s :: s in nodes ==> s.state == Phase2;
+    // requires forall s :: s in nodes ==> s.codeword[s.id] == s.symbols[s.id];
+{
+    if i == |nodes| then [] else
+    [extractSyndromes(nodes)] + syndromesToExchangeHelper(nodes, i + 1)
+}
+
+/* Helper function that generates a single seq<syndrome> for exchange. 
+* This is where Byzantine behavior can be modeled */
+function extractSyndromes(nodes: seq<Node>) : seq<syndrome> 
+    decreases nodes;
+    requires forall s :: s in nodes ==> s.n == 3*s.f + 1;
+    requires forall s :: s in nodes ==> 0 <= s.id < s.n;
+    requires forall s :: s in nodes ==> s.n == |s.symbols| == |s.codeword|;
+    requires forall s :: s in nodes ==> s.state == Phase2;
+    // requires forall s :: s in nodes ==> s.codeword[s.id] == s.symbols[s.id];
+{
+    if |nodes| == 0 then [] else
+    // assert nodes[0].codeword[nodes[0].id] == nodes[0].symbols[nodes[0].id];
+    [computeSyndrome(nodes[0])] + extractSyndromes(nodes[1..])
+    //[nodes[0].codeword[nodes[0].id]] + extractSyndromes(nodes[1..])
+}
 
 /****************************************************************************************/
 /*                                       LEMMAS                                         */
@@ -155,4 +226,82 @@ lemma  {:induction i} lemma_Exchanged_Symbols_Are_Extracted_Helper(nodes: seq<No
         lemma_Exchanged_Symbols_Are_Extracted_Helper(nodes, i+1);
     }
 }
+
+
+
+/* Proof that for any nodes: seq<Node>, |syndromesToExchange(nodes)| == |nodes| */
+lemma {:induction i} lemma_Exchange_Generates_One_SydromeSeq_For_Each_Node(nodes: seq<Node>, i:nat) 
+    decreases |nodes| - i;
+    requires 0 <= i <= |nodes|;
+    requires forall s :: s in nodes ==> |nodes| == s.n == 3*s.f + 1;
+    requires forall s :: s in nodes ==> 0 <= s.id < s.n;
+    requires forall s :: s in nodes ==> s.n == |s.symbols| == |s.codeword|;
+    requires forall s :: s in nodes ==> s.state == Phase2;
+    // requires forall s :: s in nodes ==> s.codeword[s.id] == s.symbols[s.id];
+    requires syndromesToExchangeHelper(nodes, 0) == syndromesToExchange(nodes);
+    ensures |syndromesToExchangeHelper(nodes, i)| == |nodes[i..]|;
+{
+    if i == |nodes| {
+        assert |syndromesToExchangeHelper(nodes, i)| == 0;
+    } else {
+        lemma_Exchange_Generates_One_SydromeSeq_For_Each_Node(nodes, i+1);
+    }
+}
+
+
+/* Proof that for any nodes: seq<Node>, |extractSyndromes(nodes)| == |nodes| */
+lemma {:induction nodes} lemma_Extract_Generates_One_Syndrome_For_Each_Node(nodes: seq<Node>) 
+    decreases nodes;
+    requires forall s :: s in nodes ==> s.n == 3*s.f + 1;
+    requires forall s :: s in nodes ==> 0 <= s.id < s.n;
+    requires forall s :: s in nodes ==> s.n == |s.symbols| == |s.codeword|;
+    requires forall s :: s in nodes ==> s.state == Phase2;
+    // requires forall s :: s in nodes ==> s.codeword[s.id] == s.symbols[s.id];
+    ensures |extractSyndromes(nodes)| == |nodes|;
+{
+    if |nodes| == 0 {
+        assert |extractSyndromes(nodes)| == 0;
+    } else {
+        lemma_Extract_Generates_One_Syndrome_For_Each_Node(nodes[1..]);
+    }
+}
+
+
+/* Wrapper for lemma_Exchanged_Syndromes_Are_Extracted_Helper */
+lemma {:induction nodes} lemma_Exchanged_Syndromes_Are_Extracted(nodes: seq<Node>) 
+    requires forall s :: s in nodes ==> |nodes| == s.n == 3*s.f + 1;
+    requires forall s :: s in nodes ==> 0 <= s.id < s.n;
+    requires forall s :: s in nodes ==> s.n == |s.symbols| == |s.codeword|;
+    requires forall s :: s in nodes ==> s.state == Phase2;
+    // requires forall s :: s in nodes ==> s.codeword[s.id] == s.symbols[s.id];
+    ensures |syndromesToExchange(nodes)| == |nodes|;
+    ensures |extractSyndromes(nodes)| == |nodes|;
+    ensures forall id :: 0 <= id < |syndromesToExchange(nodes)| ==> syndromesToExchange(nodes)[id] == extractSyndromes(nodes);
+{
+    lemma_Exchanged_Syndromes_Are_Extracted_Helper(nodes, 0);
+}
+
+/* Proof that every element of syndromesToExchange(nodes) is an instance of extractSyndromes(nodes) */
+lemma  {:induction i} lemma_Exchanged_Syndromes_Are_Extracted_Helper(nodes: seq<Node>, i: nat) 
+    decreases |nodes| - i;
+    requires 0 <= i <= |nodes|;
+    requires forall s :: s in nodes ==> |nodes| == s.n == 3*s.f + 1;
+    requires forall s :: s in nodes ==> 0 <= s.id < s.n;
+    requires forall s :: s in nodes ==> s.n == |s.symbols| == |s.codeword|;
+    requires forall s :: s in nodes ==> s.state == Phase2;
+    // requires forall s :: s in nodes ==> s.codeword[s.id] == s.symbols[s.id];
+    ensures |syndromesToExchange(nodes)| == |nodes|;
+    ensures |extractSyndromes(nodes)| == |nodes|;
+    ensures forall id :: 0 <= id < |syndromesToExchangeHelper(nodes, i)| ==> syndromesToExchangeHelper(nodes, i)[id] == extractSyndromes(nodes);
+{
+    lemma_Extract_Generates_One_Syndrome_For_Each_Node(nodes);
+    lemma_Exchange_Generates_One_SydromeSeq_For_Each_Node(nodes, 0);
+    if i == |nodes| {
+        assert syndromesToExchangeHelper(nodes, i) == [];
+        assert forall id :: i <= id < |syndromesToExchangeHelper(nodes, i)| ==> syndromesToExchangeHelper(nodes, i)[id] == extractSyndromes(nodes);
+    } else {
+        lemma_Exchanged_Syndromes_Are_Extracted_Helper(nodes, i+1);
+    }
+}
+
 }
